Cut dependency on FStar.Pointer in the AEAD interface

secure_api/aead/Crypto.AEAD.Main.fst
@@ -33,6 +33,8 @@ let prf_region #i #rw st = Invariant.AEADState?.log_region st //TODO: FIXME!!
 let log #i #rw s h =
   HS.sel h (Invariant.st_ilog s)
 
+let fp' = FStar.Pointer.Base.loc
+// inline_for_extraction let fp = FStar.Ghost.erased fp'
 (* let footprint #i #rw s = TSet.empty //TODO: FIXME! *)
 (* let hh_modifies_t (_:FStar.TSet.set HS.rid) (h0:HS.mem) (h1:HS.mem) = True //TODO: FIXME! *)
 let footprint #i #rw s = FStar.Ghost.hide FStar.Pointer.Base.loc_none        //TODO: FIXME!
